Progress on TopLevelRefinement... Might be out of module hell >_<.

src/coq/Handlers/Serialization.v
@@ -4,6 +4,7 @@ From Vellvm Require Import
      Numeric.Floats
      Utils.Tactics
      Utils.Util
+     Utils.OptionUtil
      Utils.Error
      Utils.ListUtil
      Utils.NonEmpty
@@ -18,7 +19,10 @@ From Vellvm Require Import
      Semantics.GepM
      Semantics.Memory.Sizeof
      Semantics.Memory.MemBytes
-     Semantics.LLVMEvents.
+     Semantics.MemoryParams
+     Semantics.LLVMEvents
+     Semantics.LLVMParams
+     Handlers.MemoryHelpers.
 
 From ExtLib Require Import
      Core.RelDec
@@ -32,391 +36,382 @@ Import IdentityMonad.
 Import ListNotations.
 Import MonadNotation.
 
-Module Make(Addr:MemoryAddress.ADDRESS)(IP:MemoryAddress.INTPTR)(SIZEOF: Sizeof)(LLVMIO: LLVM_INTERACTIONS(Addr)(IP)(SIZEOF))(PTOI:PTOI(Addr))(PROVENANCE:PROVENANCE(Addr))(ITOP:ITOP(Addr)(PROVENANCE))(GEP:GEPM(Addr)(IP)(SIZEOF)(LLVMIO))(BYTE_IMPL:ByteImpl(Addr)(IP)(SIZEOF)(LLVMIO)).
+Module Type SerializationBase (LP : LLVMParams) (Events : LLVM_INTERACTIONS LP.ADDR LP.IP LP.SIZEOF) (MP : MemoryParams LP Events).
+  Import MP.
+  Import LP.
+  Import PTOI.
+  Import ITOP.
+  Import PROV.
+  Import GEP.
+  Import SIZEOF.
+  Import Events.
 
-  Import LLVMIO.
+  Parameter ptr_size : nat.
+  Parameter endianess : Endianess.
+  Parameter concretize_uvalueM :
+    forall (M : Type -> Type) `{Monad M} (handler : dtyp -> M dvalue)
+      (ERR_M : Type -> Type) `{Monad ERR_M} `{RAISE_ERROR ERR_M} `{RAISE_UB ERR_M} `{RAISE_OOM ERR_M},
+      (forall A : Type, ERR_M A -> M A) -> uvalue -> M dvalue.
+  Parameter extractbytes_to_dvalue :
+    forall (M : Type -> Type) `{Monad M} (handler : dtyp -> M dvalue) (ERR_M : Type -> Type) `{Monad ERR_M} `{RAISE_ERROR ERR_M} `{RAISE_UB ERR_M} `{RAISE_OOM ERR_M},
+      (forall A : Type, ERR_M A -> M A) -> list uvalue -> dtyp -> M dvalue.
+
+  Parameter all_extract_bytes_from_uvalue : list uvalue -> option uvalue.
+
+  (* Equations *)
+  Parameter concretize_uvalueM_equation :
+    forall (M : Type -> Type) {HM : Monad M} (undef_handler : dtyp -> M dvalue) 
+      (ERR_M : Type -> Type) {HM_ERR : Monad ERR_M} {ERR : RAISE_ERROR ERR_M} {UB : RAISE_UB ERR_M}
+      {OOM : RAISE_OOM ERR_M} (lift_ue : forall A : Type, ERR_M A -> M A) (u : uvalue),
+      concretize_uvalueM M undef_handler ERR_M lift_ue u =
+        match u with
+        | UVALUE_Addr a => ret (DVALUE_Addr a)
+        | UVALUE_I1 x => ret (DVALUE_I1 x)
+        | UVALUE_I8 x => ret (DVALUE_I8 x)
+        | UVALUE_I32 x => ret (DVALUE_I32 x)
+        | UVALUE_I64 x => ret (DVALUE_I64 x)
+        | UVALUE_IPTR x => ret (DVALUE_IPTR x)
+        | UVALUE_Double x => ret (DVALUE_Double x)
+        | UVALUE_Float x => ret (DVALUE_Float x)
+        | UVALUE_Undef t => undef_handler t
+        | UVALUE_Poison t => ret (DVALUE_Poison t)
+        | UVALUE_None => ret DVALUE_None
+        | UVALUE_Struct fields =>
+            x <- map_monad (concretize_uvalueM M undef_handler ERR_M lift_ue) fields;; ret (DVALUE_Struct x)
+        | UVALUE_Packed_struct fields =>
+            x <- map_monad (concretize_uvalueM M undef_handler ERR_M lift_ue) fields;;
+            ret (DVALUE_Packed_struct x)
+        | UVALUE_Array elts =>
+            x <- map_monad (concretize_uvalueM M undef_handler ERR_M lift_ue) elts;; ret (DVALUE_Array x)
+        | UVALUE_Vector elts =>
+            x <- map_monad (concretize_uvalueM M undef_handler ERR_M lift_ue) elts;; ret (DVALUE_Vector x)
+        | UVALUE_IBinop iop v1 v2 =>
+            dv1 <- concretize_uvalueM M undef_handler ERR_M lift_ue v1;;
+            dv2 <- concretize_uvalueM M undef_handler ERR_M lift_ue v2;; lift_ue dvalue (eval_iop iop dv1 dv2)
+        | UVALUE_ICmp cmp v1 v2 =>
+            dv1 <- concretize_uvalueM M undef_handler ERR_M lift_ue v1;;
+            dv2 <- concretize_uvalueM M undef_handler ERR_M lift_ue v2;; lift_ue dvalue (eval_icmp cmp dv1 dv2)
+        | UVALUE_FBinop fop _ v1 v2 =>
+            dv1 <- concretize_uvalueM M undef_handler ERR_M lift_ue v1;;
+            dv2 <- concretize_uvalueM M undef_handler ERR_M lift_ue v2;; lift_ue dvalue (eval_fop fop dv1 dv2)
+        | UVALUE_FCmp cmp v1 v2 =>
+            dv1 <- concretize_uvalueM M undef_handler ERR_M lift_ue v1;;
+            dv2 <- concretize_uvalueM M undef_handler ERR_M lift_ue v2;; lift_ue dvalue (eval_fcmp cmp dv1 dv2)
+        | UVALUE_Conversion conv t_from v t_to =>
+            dv <- concretize_uvalueM M undef_handler ERR_M lift_ue v;;
+            match get_conv_case conv t_from dv t_to with
+            | Conv_Pure x => ret x
+            | Conv_ItoP x => ret (DVALUE_Addr (int_to_ptr (dvalue_int_unsigned x) wildcard_prov))
+            | Conv_PtoI (DVALUE_Addr addr) =>
+                match t_to with
+                | DTYPE_I sz => lift_ue dvalue (coerce_integer_to_int (Some sz) (ptr_to_int addr))
+                | DTYPE_IPTR => lift_ue dvalue (coerce_integer_to_int None (ptr_to_int addr))
+                | _ => lift_ue dvalue (raise_error "Invalid PTOI conversion")
+                end
+            | Conv_Illegal s => lift_ue dvalue (raise_error s)
+            | _ => lift_ue dvalue (raise_error "Invalid PTOI conversion")
+            end
+        | UVALUE_GetElementPtr t ua uvs =>
+            da <- concretize_uvalueM M undef_handler ERR_M lift_ue ua;;
+            dvs <- map_monad (concretize_uvalueM M undef_handler ERR_M lift_ue) uvs;;
+            match handle_gep t da dvs with
+            | inl err => lift_ue dvalue (raise_error err)
+            | inr dv => ret dv
+            end
+        | UVALUE_ExtractValue uv idxs =>
+            str <- concretize_uvalueM M undef_handler ERR_M lift_ue uv;;
+            (let
+                fix loop (str0 : dvalue) (idxs0 : list int) {struct idxs0} : ERR_M dvalue :=
+                match idxs0 with
+                | [] => ret str0
+                | i :: tl => v <- index_into_str_dv str0 i;; loop v tl
+                end in
+              lift_ue dvalue (loop str idxs))
+        | UVALUE_Select cond v1 v2 =>
+            dcond <- concretize_uvalueM M undef_handler ERR_M lift_ue cond;;
+            uv <- lift_ue uvalue (eval_select dcond v1 v2);;
+            concretize_uvalueM M undef_handler ERR_M lift_ue uv
+        | UVALUE_ExtractByte _ _ _ _ =>
+            lift_ue dvalue (raise_error "Attempting to concretize UVALUE_ExtractByte, should not happen.")
+        | UVALUE_ConcatBytes bytes dt =>
+            if N.of_nat (Datatypes.length bytes) =? sizeof_dtyp dt
+            then
+              match all_extract_bytes_from_uvalue bytes with
+              | Some uv => concretize_uvalueM M undef_handler ERR_M lift_ue uv
+              | None => extractbytes_to_dvalue M undef_handler ERR_M lift_ue bytes dt
+              end
+            else extractbytes_to_dvalue M undef_handler ERR_M lift_ue bytes dt
+        | _ =>
+            lift_ue dvalue
+                    (raise_error
+                       ("concretize_uvalueM: Attempting to convert a partially non-reduced uvalue to dvalue. Should not happen: " ++
+                                                                                                                                  uvalue_constructor_string u))
+        end.
+End SerializationBase.
+
+Module Type Serialization (LP : LLVMParams) (Events : LLVM_INTERACTIONS LP.ADDR LP.IP LP.SIZEOF) (MP : MemoryParams LP Events) (SER : SerializationBase LP Events MP) <: SerializationBase LP Events MP.
+  Include SER.
+  Import MP.
+  Import LP.
+  Import Events.
+
+  Definition concretize_uvalue {M} `{Monad M} `{RAISE_ERROR M} `{RAISE_UB M} `{RAISE_OOM M}
+             (uv : uvalue) : M dvalue
+    := concretize_uvalueM M (fun dt => lift_err_RAISE_ERROR (default_dvalue_of_dtyp dt)) M (fun _ x => x) uv.
+
+  Definition concretize_u (uv : uvalue) : RefineProp dvalue.
+    refine (concretize_uvalueM _ (fun dt => _) err_ub_oom (fun _ x => _) uv).
+
+    (* Undef handler *)
+    { unfold RefineProp.
+      refine (fun edv => match unERR_UB_OOM edv with
+                      | mkEitherT (mkEitherT (mkEitherT (mkIdent (inr (inr (inr dv)))))) =>
+                          (* As long as the dvalue has the same type, it's a refinement *)
+                          dvalue_has_dtyp dv dt
+                      | _ => False
+                      end).
+    }
+
+    (* lift_ue *)
+    { unfold RefineProp.
+      intros ue.
+
+      (* Is x or ue the thing that should be the refinement? *)
+      (* I think ue is the refinement *)
+      destruct x as [[[[[[[oom_x] | [[ub_x] | [[err_x] | x]]]]]]]].
+      - (* OOM *)
+        (* OOM only refines OOM *)
+        destruct ue as [[[[[[[oom_ue] | [[ub_ue] | [[err_ue] | ue]]]]]]]].
+        + exact True.
+        + exact False.
+        + exact False.
+        + exact False.
+      - (* UB *)
+        exact True.
+      - (* ERR *)
+        exact True.
+      - destruct ue as [[[[[[[oom_ue] | [[ub_ue] | [[err_ue] | ue]]]]]]]].
+        + exact True. (* OOM refines everything *)
+        + exact False.
+        + exact False.
+        + exact (x = ue).
+    }
+  Defined.
+
+  Definition concretize_u_succeeds (uv : uvalue) : RefineProp dvalue.
+    refine (concretize_uvalueM _ (fun dt => _) err_ub_oom (fun _ x => _) uv).
+
+    (* Undef handler *)
+    { unfold RefineProp.
+      refine (fun edv => match unERR_UB_OOM edv with
+                      | mkEitherT (mkEitherT (mkEitherT (mkIdent (inr (inr (inr dv)))))) =>
+                          (* As long as the dvalue has the same type, it's a refinement *)
+                          dvalue_has_dtyp dv dt
+                      | _ => False
+                      end).
+    }
+
+    (* lift_ue *)
+    { unfold RefineProp.
+      intros ue.
+
+      exact (~MFails x /\ ~MFails ue).
+    }
+  Defined.
+
+  Definition concretize (uv: uvalue) (dv : dvalue) := concretize_u uv (ret dv).
+
+  Definition concretize_fails (uv : uvalue) : Prop
+    := concretize_u uv (raise_ub "").
+
+  Definition concretize_succeeds (uv : uvalue) : Prop
+    := ~ concretize_fails uv.
+
+  Lemma concretize_equation : forall (uv: uvalue) (dv : dvalue),
+      concretize uv dv = concretize_u uv (ret dv).
+  Proof.
+    reflexivity.
+  Qed.
+
+  Lemma Concretize_Undef : forall dt dv,
+      dvalue_has_dtyp dv dt ->
+      concretize (UVALUE_Undef dt) dv.
+  Proof.
+    intros dt dv H.
+    rewrite concretize_equation.
+    unfold concretize_u.
+    rewrite concretize_uvalueM_equation.
+    cbn; auto.
+  Qed.
+
+  Lemma Concretize_IBinop : forall iop uv1 e1 uv2 e2,
+      concretize_u uv1 e1 ->
+      concretize_u uv2 e2 ->
+      concretize_u (UVALUE_IBinop iop uv1 uv2)
+                   (dv1 <- e1 ;;
+                    dv2 <- e2 ;;
+                    (eval_iop iop dv1 dv2)).
+  Proof.
+    intros iop uv1 e1 uv2 e2 C1 C2.
+    unfold concretize_u in *.
+
+    rewrite concretize_uvalueM_equation.
+    red.
+
+    unfold bind.
+    cbn.
+    unfold bind_RefineProp.
+
+    eexists.
+    exists (fun x => match unIdent (unEitherT (unEitherT (unEitherT (unERR_UB_OOM e2)))) with
+             | inl (OOM_message oom) => raise_oom oom
+             | inr (inl (UB_message ub)) => raise_ub ub
+             | inr (inr (inl (ERR_message err))) => raise_error err
+             | inr (inr (inr x0)) => eval_iop iop x x0
+             end).
+    split; eauto.
+    split.
+
+    { (* Monad.eq1 mb (x <- ma;; k' x) *)
+      unfold bind.
+      cbn.
+      destruct e1 as [[[[[[[oom_e1] | [[ub_e1] | [[err_e1] | e1]]]]]]]]; cbn; try reflexivity.
+      destruct e2 as [[[[[[[oom_e2] | [[ub_e2] | [[err_e2] | e2]]]]]]]]; cbn; try reflexivity.
+
+      destruct (eval_iop iop e1 e2) as [[[[[[[oom_eval_iopiope1e2] | [[ub_eval_iopiope1e2] | [[err_eval_iopiope1e2] | eval_iopiope1e2]]]]]]]]; reflexivity.
+    }
+
+    right.
+    intros dv1 Re1.
+
+    eexists.
+    exists (fun x0 => eval_iop iop dv1 x0).
+    split; eauto.
+    split.
+
+    { (* Monad.eq1 mb (x <- ma;; k' x) *)
+      unfold bind.
+      cbn.
+      destruct e2 as [[[[[[[oom_e2] | [[ub_e2] | [[err_e2] | e2]]]]]]]]; cbn; try reflexivity.
+
+      unfold Monad.eq1.
+      destruct (eval_iop iop dv1 e2) as [[[[[[[oom_eval_iopiopdv1e2] | [[ub_eval_iopiopdv1e2] | [[err_eval_iopiopdv1e2] | eval_iopiopdv1e2]]]]]]]]; reflexivity.
+    }
+
+    right.
+    intros dv2 Re2.
+    destruct (eval_iop iop dv1 dv2) as [[[[[[[oom_eval_iopiopdv1dv2] | [[ub_eval_iopiopdv1dv2] | [[err_eval_iopiopdv1dv2] | eval_iopiopdv1dv2]]]]]]]]; reflexivity.
+  Qed.
+End Serialization.
+
+Module MakeBase (LP : LLVMParams) (Events : LLVM_INTERACTIONS LP.ADDR LP.IP LP.SIZEOF) (MP : MemoryParams LP Events) : SerializationBase LP Events MP.
+  Import MP.
+  Import LP.
+  Import Events.
   Import SIZEOF.
   Import PTOI.
-  Import PROVENANCE.
+  Import PROV.
   Import ITOP.
   Import DV.
   Import GEP.
   Open Scope list.
 
-  Module BYTE := Byte Addr IP SIZEOF LLVMIO BYTE_IMPL.
+  Module BYTE := Byte ADDR IP SIZEOF Events BYTE_IMPL.
   Export BYTE.
 
   (* Variable ptr_size : nat. *)
   (* Variable datalayout : DataLayout. *)
   Definition ptr_size : nat := 8.
 
-  Definition addr := Addr.addr.
+  Definition addr := ADDR.addr.
 
-  (* TODO: parameterize *)
   Definition endianess : Endianess
     := ENDIAN_LITTLE.
 
-  (* Given a little endian list of bytes, match the endianess of `e` *)
-  Definition correct_endianess {BYTES : Type} (e : Endianess) (bytes : list BYTES)
-    := match e with
-       | ENDIAN_BIG => rev bytes
-       | ENDIAN_LITTLE => bytes
-       end.
-
-    (* Is a uvalue a concrete integer equal to i? *)
-    Definition uvalue_int_eq_Z (uv : uvalue) (i : Z)
-      := match uv with
-         | UVALUE_I1 x
-         | UVALUE_I8 x
-         | UVALUE_I32 x
-         | UVALUE_I64 x => Z.eqb (unsigned x) i
-         | UVALUE_IPTR x => Z.eqb (IP.to_Z x) i
-         | _ => false
-         end.
-
-    Definition dvalue_int_unsigned (dv : dvalue) : Z
-      := match dv with
-         | DVALUE_I1 x => unsigned x
-         | DVALUE_I8 x => unsigned x
-         | DVALUE_I32 x => unsigned x
-         | DVALUE_I64 x => unsigned x
-         | DVALUE_IPTR x => IP.to_Z x (* TODO: unsigned???? *)
-         | _ => 0
-         end.
-
-    Definition guard_opt (x : bool) : option unit
-      := if x then Some tt else None.
-
-    (* TODO: move this *)
-    Definition dtyp_eqb (dt1 dt2 : dtyp) : bool
-      := match @dtyp_eq_dec dt1 dt2 with
-         | left x => true
-         | right x => false
-         end.
-
-    Fixpoint all_extract_bytes_from_uvalue_helper (idx' : Z) (sid' : store_id) (dt' : dtyp) (parent : uvalue) (bytes : list uvalue) : option uvalue
-      := match bytes with
-         | [] => Some parent
-         | (UVALUE_ExtractByte uv dt idx sid)::bytes =>
+  Fixpoint all_extract_bytes_from_uvalue_helper (idx' : Z) (sid' : store_id) (dt' : dtyp) (parent : uvalue) (bytes : list uvalue) : option uvalue
+    := match bytes with
+       | [] => Some parent
+       | (UVALUE_ExtractByte uv dt idx sid)::bytes =>
            guard_opt (uvalue_int_eq_Z idx idx');;
            guard_opt (RelDec.rel_dec uv parent);;
            guard_opt (N.eqb sid sid');;
            guard_opt (dtyp_eqb dt dt');;
            all_extract_bytes_from_uvalue_helper (Z.succ idx') sid' dt' parent bytes
-         | _ => None
-         end.
+       | _ => None
+       end.
 
-    (* Check that store ids, uvalues, and types match up, as well as
+  (* Check that store ids, uvalues, and types match up, as well as
        that the extract byte indices are in the right order *)
-    Definition all_extract_bytes_from_uvalue (bytes : list uvalue) : option uvalue
-      := match bytes with
-         | nil => None
-         | (UVALUE_ExtractByte uv dt idx sid)::xs =>
+  Definition all_extract_bytes_from_uvalue (bytes : list uvalue) : option uvalue
+    := match bytes with
+       | nil => None
+       | (UVALUE_ExtractByte uv dt idx sid)::xs =>
            all_extract_bytes_from_uvalue_helper 0 sid dt uv bytes
-         | _ => None
-         end.
+       | _ => None
+       end.
 
-    (* TODO: move to utils? *)
-    Definition from_option {A} (def : A) (opt : option A) : A
-      := match opt with
-         | Some x => x
-         | None => def
-         end.
+  (* Definition fp_alignment (bits : N) : option Alignment := *)
+  (*   let fp_map := dl_floating_point_alignments datalayout *)
+  (*   in NM.find bits fp_map. *)
 
-    (* Definition fp_alignment (bits : N) : option Alignment := *)
-    (*   let fp_map := dl_floating_point_alignments datalayout *)
-    (*   in NM.find bits fp_map. *)
+  (* Definition int_alignment (bits : N) : option Alignment := *)
+  (*   let int_map := dl_integer_alignments datalayout *)
+  (*   in match NM.find bits int_map with *)
+  (*      | Some align => Some align *)
+  (*      | None => *)
+  (*        let keys  := map fst (NM.elements int_map) in *)
+  (*        let bits' := nextOrMaximumOpt N.leb bits keys  *)
+  (*        in match bits' with *)
+  (*           | Some bits => NM.find bits int_map *)
+  (*           | None => None *)
+  (*           end *)
+  (*      end. *)
 
-    Definition option_pick_large {A} (leq : A -> A -> bool) (a b : option A) : option A
-      := match a, b with
-         | Some x, Some y =>
-           if leq x y then b else a
-         | Some a, _      => Some a
-         | _, Some b      => Some b
-         | None, None     => None
-         end.
+  (* TODO: Finish this function *)
+  (* Fixpoint dtyp_alignment (dt : dtyp) : option Alignment := *)
+  (*   match dt with *)
+  (*   | DTYPE_I sz => *)
+  (*     int_alignment sz *)
+  (*   | DTYPE_IPTR => *)
+  (*     (* TODO: should these have the same alignments as pointers? *) *)
+  (*     int_alignment (N.of_nat ptr_size * 4)%N *)
+  (*   | DTYPE_Pointer => *)
+  (*     (* TODO: address spaces? *) *)
+  (*     Some (ps_alignment (head (dl_pointer_alignments datalayout))) *)
+  (*   | DTYPE_Void => *)
+  (*     None *)
+  (*   | DTYPE_Half => *)
+  (*     fp_alignment 16 *)
+  (*   | DTYPE_Float => *)
+  (*     fp_alignment 32 *)
+  (*   | DTYPE_Double => *)
+  (*     fp_alignment 64 *)
+  (*   | DTYPE_X86_fp80 => *)
+  (*     fp_alignment 80 *)
+  (*   | DTYPE_Fp128 => *)
+  (*     fp_alignment 128 *)
+  (*   | DTYPE_Ppc_fp128 => *)
+  (*     fp_alignment 128 *)
+  (*   | DTYPE_Metadata => *)
+  (*     None *)
+  (*   | DTYPE_X86_mmx => _ *)
+  (*   | DTYPE_Array sz t => *)
+  (*     dtyp_alignment t *)
+  (*   | DTYPE_Struct fields => _ *)
+  (*   | DTYPE_Packed_struct fields => _ *)
+  (*   | DTYPE_Opaque => _ *)
+  (*   | DTYPE_Vector sz t => _ *)
+  (*   end. *)
 
-    Definition option_pick_small {A} (leq : A -> A -> bool) (a b : option A) : option A
-      := match a, b with
-         | Some x, Some y =>
-           if leq x y then a else b
-         | Some a, _      => Some a
-         | _, Some b      => Some b
-         | None, None     => None
-         end.
+  (* Assign fresh sids to ubytes while preserving entanglement *)
 
-    Definition maximumBy {A} (leq : A -> A -> bool) (def : A) (l : list A) : A :=
-      fold_left (fun a b => if leq a b then b else a) l def.
-
-    Definition maximumByOpt {A} (leq : A -> A -> bool) (l : list A) : option A :=
-      fold_left (option_pick_large leq) (map Some l) None.
-
-    Definition nextLargest {A} (leq : A -> A -> bool) (n : A) (def : A) (l : list A) : A :=
-      fold_left (fun a b => if leq n a && leq a b then a else b) l def.
-
-    Definition nextOrMaximum {A} (leq : A -> A -> bool) (n : A) (def : A) (l : list A) : A :=
-      let max := maximumBy leq def l
-      in fold_left (fun a b => if leq n b && leq a b then a else b) l max.
-
-    Definition nextOrMaximumOpt {A} (leq : A -> A -> bool) (n : A) (l : list A) : option A :=
-      let max := maximumByOpt leq l
-      in fold_left (fun a b => if leq n b then option_pick_small leq a (Some b) else a) l max.
-
-    (* Definition int_alignment (bits : N) : option Alignment := *)
-    (*   let int_map := dl_integer_alignments datalayout *)
-    (*   in match NM.find bits int_map with *)
-    (*      | Some align => Some align *)
-    (*      | None => *)
-    (*        let keys  := map fst (NM.elements int_map) in *)
-    (*        let bits' := nextOrMaximumOpt N.leb bits keys  *)
-    (*        in match bits' with *)
-    (*           | Some bits => NM.find bits int_map *)
-    (*           | None => None *)
-    (*           end *)
-    (*      end. *)
-
-    (* TODO: Finish this function *)
-    (* Fixpoint dtyp_alignment (dt : dtyp) : option Alignment := *)
-    (*   match dt with *)
-    (*   | DTYPE_I sz => *)
-    (*     int_alignment sz *)
-    (*   | DTYPE_IPTR => *)
-    (*     (* TODO: should these have the same alignments as pointers? *) *)
-    (*     int_alignment (N.of_nat ptr_size * 4)%N *)
-    (*   | DTYPE_Pointer => *)
-    (*     (* TODO: address spaces? *) *)
-    (*     Some (ps_alignment (head (dl_pointer_alignments datalayout))) *)
-    (*   | DTYPE_Void => *)
-    (*     None *)
-    (*   | DTYPE_Half => *)
-    (*     fp_alignment 16 *)
-    (*   | DTYPE_Float => *)
-    (*     fp_alignment 32 *)
-    (*   | DTYPE_Double => *)
-    (*     fp_alignment 64 *)
-    (*   | DTYPE_X86_fp80 => *)
-    (*     fp_alignment 80 *)
-    (*   | DTYPE_Fp128 => *)
-    (*     fp_alignment 128 *)
-    (*   | DTYPE_Ppc_fp128 => *)
-    (*     fp_alignment 128 *)
-    (*   | DTYPE_Metadata => *)
-    (*     None *)
-    (*   | DTYPE_X86_mmx => _ *)
-    (*   | DTYPE_Array sz t => *)
-    (*     dtyp_alignment t *)
-    (*   | DTYPE_Struct fields => _ *)
-    (*   | DTYPE_Packed_struct fields => _ *)
-    (*   | DTYPE_Opaque => _ *)
-    (*   | DTYPE_Vector sz t => _ *)
-    (*   end. *)
-
-    (* Assign fresh sids to ubytes while preserving entanglement *)
-    Definition default_dvalue_of_dtyp_i (sz : N) : err dvalue:=
-      (if (sz =? 64) then ret (DVALUE_I64 (repr 0))
-        else if (sz =? 32) then ret (DVALUE_I32 (repr 0))
-            else if (sz =? 8) then ret (DVALUE_I8 (repr 0))
-                  else if (sz =? 1) then ret (DVALUE_I1 (repr 0))
-                       else failwith
-              "Illegal size for generating default dvalue of DTYPE_I").
-
-
-    (* Handler for PickE which concretizes everything to 0 *)
-    Fixpoint default_dvalue_of_dtyp (dt : dtyp) : err dvalue :=
-      match dt with
-      | DTYPE_I sz => default_dvalue_of_dtyp_i sz
-      | DTYPE_IPTR => ret (DVALUE_IPTR IP.zero)
-      | DTYPE_Pointer => ret (DVALUE_Addr Addr.null)
-      | DTYPE_Void => ret DVALUE_None
-      | DTYPE_Half => failwith "Unimplemented default type: half"
-      | DTYPE_Float => ret (DVALUE_Float Float32.zero)
-      | DTYPE_Double => ret (DVALUE_Double (Float32.to_double Float32.zero))
-      | DTYPE_X86_fp80 => failwith "Unimplemented default type: x86_fp80"
-      | DTYPE_Fp128 => failwith "Unimplemented default type: fp128"
-      | DTYPE_Ppc_fp128 => failwith "Unimplemented default type: ppc_fp128"
-      | DTYPE_Metadata => failwith "Unimplemented default type: metadata"
-      | DTYPE_X86_mmx => failwith "Unimplemented default type: x86_mmx"
-      | DTYPE_Opaque => failwith "Unimplemented default type: opaque"
-      | DTYPE_Array sz t =>
-        if (0 <=? sz) then
-          v <- default_dvalue_of_dtyp t ;;
-          (ret (DVALUE_Array (repeat v (N.to_nat sz))))
-        else
-          failwith ("Negative array length for generating default value" ++
-          "of DTYPE_Array or DTYPE_Vector")
-
-      (* Matching valid Vector types... *)
-      (* Currently commented out unsupported ones *)
-      (* | DTYPE_Vector sz (DTYPE_Half) => *)
-      (*   if (0 <=? sz) then *)
-      (*     (ret (DVALUE_Vector *)
-      (*             (repeat (DVALUE_Float Float32.zero) (N.to_nat sz)))) *)
-      (*   else *)
-      (*     failwith ("Negative array length for generating default value" ++ *)
-      (*     "of DTYPE_Array or DTYPE_Vector") *)
-      | DTYPE_Vector sz (DTYPE_Float) =>
-        if (0 <=? sz) then
-          (ret (DVALUE_Vector
-                  (repeat (DVALUE_Float Float32.zero) (N.to_nat sz))))
-        else
-          failwith ("Negative array length for generating default value" ++
-          "of DTYPE_Array or DTYPE_Vector")
-      | DTYPE_Vector sz (DTYPE_Double) =>
-        if (0 <=? sz) then
-          (ret (DVALUE_Vector
-                  (repeat (DVALUE_Double (Float32.to_double Float32.zero))
-                          (N.to_nat sz))))
-        else
-          failwith ("Negative array length for generating default value" ++
-          "of DTYPE_Array or DTYPE_Vector")
-      (* | DTYPE_Vector sz (DTYPE_X86_fp80) => *)
-      (*   if (0 <=? sz) then *)
-      (*     (ret (DVALUE_Vector *)
-      (*             (repeat (DVALUE_Float Float32.zero) (N.to_nat sz)))) *)
-      (*   else *)
-      (*     failwith ("Negative array length for generating default value" ++ *)
-      (*     "of DTYPE_Array or DTYPE_Vector") *)
-      (* | DTYPE_Vector sz (DTYPE_Fp128) => *)
-      (*   if (0 <=? sz) then *)
-      (*     (ret (DVALUE_Vector *)
-      (*             (repeat (DVALUE_Float Float32.zero) (N.to_nat sz)))) *)
-      (*   else *)
-      (*     failwith ("Negative array length for generating default value" ++ *)
-      (*     "of DTYPE_Array or DTYPE_Vector") *)
-      | DTYPE_Vector sz (DTYPE_I n) =>
-        if (0 <=? sz) then
-          v <- default_dvalue_of_dtyp_i n ;;
-          (ret (DVALUE_Vector (repeat v (N.to_nat sz))))
-        else
-          failwith ("Negative array length for generating default value" ++
-          "of DTYPE_Array or DTYPE_Vector")
-      | DTYPE_Vector _ _ => failwith ("Non-valid vector type when" ++
-          "generating default vector")
-      | DTYPE_Struct fields =>
-        v <- @map_monad err _ dtyp dvalue default_dvalue_of_dtyp fields;;
-        ret (DVALUE_Struct v)
-      | DTYPE_Packed_struct fields =>
-        v <- @map_monad err _ dtyp dvalue default_dvalue_of_dtyp fields;;
-        ret (DVALUE_Packed_struct v)
-      end.
-
-    Ltac do_it := constructor; cbn; auto; fail.
-
-    Lemma dvalue_default : forall t v,
-        inr v = (default_dvalue_of_dtyp t) ->
-        dvalue_has_dtyp v t.
-    Proof.
-      intros t v. revert v.
-      induction t; try do_it;
-        try (intros; subst; inversion H; constructor).
-      - intros. subst. cbn in H.
-        unfold default_dvalue_of_dtyp_i in H.
-        destruct (@IX_supported_dec a).
-        * inversion i; subst; cbn in H; inversion H; constructor; auto.
-        * rewrite unsupported_cases in H; auto. inversion H.
-      - intros. subst. inversion H. clear H.
-        induction sz.
-        + cbn in H1.
-          destruct (default_dvalue_of_dtyp t) eqn: HT. inv H1. inv H1.
-          pose proof DVALUE_Array_typ.
-          specialize (H nil (N.to_nat 0) t).
-          rewrite Nnat.N2Nat.id in H.
-          apply H. auto. auto.
-        + cbn in H1.
-          destruct (default_dvalue_of_dtyp t) eqn: HT. inv H1. inv H1.
-          pose proof DVALUE_Array_typ as ARR.
-          specialize (ARR (repeat d (Pos.to_nat p)) (N.to_nat (N.pos p)) t).
-          rewrite Nnat.N2Nat.id in ARR.
-          cbn in *.
-          apply ARR.
-          * apply forall_repeat_true.
-            apply IHt. reflexivity.
-          * apply repeat_length.
-      - revert H. induction fields.
-        + intros. inv H0. constructor.
-        + intros.
-          assert (forall u : dtyp,
-              In u fields ->
-              forall v : dvalue,
-                inr v = default_dvalue_of_dtyp u -> dvalue_has_dtyp v u).
-          { intros. apply H. apply in_cons. auto. auto. }
-          specialize (IHfields H1). clear H1.
-          Opaque map_monad.
-          (* Reduce H0 *)
-          cbn in H0.
-          rewrite list_cons_app in H0.
-          rewrite map_monad_app in H0. cbn in H0.
-          Transparent map_monad.
-          unfold map_monad at 1 in H0.
-          Opaque map_monad. cbn in H0.
-          destruct (default_dvalue_of_dtyp a) eqn: A_DEFAULT.
-          inv H0.
-          destruct (map_monad default_dvalue_of_dtyp fields) eqn: FIELDS.
-          inv H0.
-          inv H0. constructor. apply H. apply in_eq.
-          symmetry. auto.
-          apply IHfields. cbn. rewrite FIELDS. reflexivity.
-      - revert H. induction fields.
-        + intros. inv H0. constructor.
-        + intros.
-          assert (forall u : dtyp,
-              In u fields ->
-              forall v : dvalue,
-                inr v = default_dvalue_of_dtyp u -> dvalue_has_dtyp v u).
-          { intros. apply H. apply in_cons. auto. auto. }
-          specialize (IHfields H1). clear H1.
-          Opaque map_monad.
-          (* Reduce H0 *)
-          cbn in H0.
-          rewrite list_cons_app in H0.
-          rewrite map_monad_app in H0. cbn in H0.
-          Transparent map_monad.
-          unfold map_monad at 1 in H0.
-          Opaque map_monad. cbn in H0.
-          destruct (default_dvalue_of_dtyp a) eqn: A_DEFAULT.
-          inv H0.
-          destruct (map_monad default_dvalue_of_dtyp fields) eqn: FIELDS.
-          inv H0.
-          inv H0. constructor. apply H. apply in_eq.
-          symmetry. auto.
-          apply IHfields. cbn. rewrite FIELDS. reflexivity.
-      - intros. subst. inversion H. clear H.
-        revert H1. revert v. revert IHt. revert t.
-        induction sz.
-        + intros. cbn in H1.
-          pose proof DVALUE_Vector_typ.
-          specialize (H nil (N.to_nat 0)).
-          rewrite Nnat.N2Nat.id in H.
-          destruct t; inv H1;
-              try
-                (apply H;
-                 [constructor | constructor |
-                  unfold vector_dtyp; intuition]).
-          destruct (default_dvalue_of_dtyp_i sz) eqn: HI; inv H2.
-          apply H. constructor. auto. unfold vector_dtyp. left.
-          exists sz. reflexivity.
-        + intros. cbn in H1.
-          destruct t; inv H1;
-            try (
-                rewrite <- positive_nat_N;
-                   constructor; [apply forall_repeat_true ; constructor |
-                          apply repeat_length |
-                          unfold vector_dtyp ; intuition ]).
-          destruct (default_dvalue_of_dtyp_i sz) eqn: SZ; inv H0.
-            pose proof DVALUE_Vector_typ.
-            rewrite <- positive_nat_N. apply H.
-            apply forall_repeat_true. apply IHt. symmetry. auto.
-            apply repeat_length.
-            left. exists sz. reflexivity.
-    Qed.
-
-    Section Concretize.
+  Section Concretize.
 
 
 
-      Variable endianess : Endianess.
+    Variable endianess : Endianess.
 
-      (* Convert a list of UVALUE_ExtractByte values into a dvalue of
+    (* Convert a list of UVALUE_ExtractByte values into a dvalue of
          a given type.
 
          Assumes bytes are in little endian form...
@@ -452,420 +447,387 @@ Module Make(Addr:MemoryAddress.ADDRESS)(IP:MemoryAddress.INTPTR)(SIZEOF: Sizeof)
          convert the corresponding byte extractions into a single
          dvalue.
 
-       *)
+     *)
 
-      (* TODO: probably move this *)
-      (* TODO: Make these take endianess into account.
+    (* TODO: probably move this *)
+    (* TODO: Make these take endianess into account.
 
          Can probably use bitwidth from VInt to do big-endian...
-       *)
-      Definition extract_byte_vint {I} `{VInt I} (i : I) (idx : Z) : Z
-        := unsigned (modu (shru i (repr (idx * 8))) (repr 256)).
+     *)
+    Definition extract_byte_vint {I} `{VInt I} (i : I) (idx : Z) : Z
+      := unsigned (modu (shru i (repr (idx * 8))) (repr 256)).
 
-      Fixpoint concat_bytes_vint {I} `{VInt I} (bytes : list I) : I
-        := match bytes with
-           | [] => repr 0
-           | (byte::bytes) =>
+    Fixpoint concat_bytes_vint {I} `{VInt I} (bytes : list I) : I
+      := match bytes with
+         | [] => repr 0
+         | (byte::bytes) =>
              add byte (shl (concat_bytes_vint bytes) (repr 8))
-           end.
+         end.
 
-      (* TODO: Endianess *)
-      (* TODO: does this work correctly with negative x? *)
-      Definition extract_byte_Z (x : Z) (idx : Z) : Z
-        := (Z.shiftr x (idx * 8)) mod 256.
+    (* TODO: Endianess *)
+    (* TODO: does this work correctly with negative x? *)
+    Definition extract_byte_Z (x : Z) (idx : Z) : Z
+      := (Z.shiftr x (idx * 8)) mod 256.
 
-      (* TODO: Endianess *)
-      Definition concat_bytes_Z_vint {I} `{VInt I} (bytes : list Z) : I
-        := concat_bytes_vint (map repr bytes).
+    (* TODO: Endianess *)
+    Definition concat_bytes_Z_vint {I} `{VInt I} (bytes : list Z) : I
+      := concat_bytes_vint (map repr bytes).
 
-      (* TODO: Endianess *)
-      Fixpoint concat_bytes_Z (bytes : list Z) : Z
-        := match bytes with
-           | [] => 0
-           | (byte::bytes) =>
+    (* TODO: Endianess *)
+    Fixpoint concat_bytes_Z (bytes : list Z) : Z
+      := match bytes with
+         | [] => 0
+         | (byte::bytes) =>
              byte + (Z.shiftl (concat_bytes_Z bytes) 8)
-           end.
+         end.
 
-      (* TODO: Move this??? *)
-      Inductive Poisonable (A : Type) : Type :=
-      | Unpoisoned : A -> Poisonable A
-      | Poison : forall (dt : dtyp), Poisonable A
-      .
+    (* TODO: Move this??? *)
+    Inductive Poisonable (A : Type) : Type :=
+    | Unpoisoned : A -> Poisonable A
+    | Poison : forall (dt : dtyp), Poisonable A
+    .
 
-      Arguments Unpoisoned {A} a.
-      Arguments Poison {A}.
+    Arguments Unpoisoned {A} a.
+    Arguments Poison {A}.
 
-      Global Instance MonadPoisonable : Monad Poisonable
-        := { ret  := @Unpoisoned;
-             bind := fun _ _ ma mab => match ma with
-                                    | Poison dt => Poison dt
-                                    | Unpoisoned v => mab v
-                                    end
-        }.
+    Global Instance MonadPoisonable : Monad Poisonable
+      := { ret  := @Unpoisoned;
+           bind := fun _ _ ma mab => match ma with
+                                     | Poison dt => Poison dt
+                                     | Unpoisoned v => mab v
+                                     end
+      }.
 
-      Class RAISE_POISON (M : Type -> Type) :=
-        { raise_poison : forall {A}, dtyp -> M A }.
+    Class RAISE_POISON (M : Type -> Type) :=
+      { raise_poison : forall {A}, dtyp -> M A }.
 
-      Global Instance RAISE_POISON_Poisonable : RAISE_POISON Poisonable :=
-        { raise_poison := fun A dt => Poison dt }.
+    Global Instance RAISE_POISON_Poisonable : RAISE_POISON Poisonable :=
+      { raise_poison := fun A dt => Poison dt }.
 
-      #[global] Instance RAISE_POISON_E_MT {M : Type -> Type} {MT : (Type -> Type) -> Type -> Type} `{MonadT (MT M) M} `{RAISE_POISON M} : RAISE_POISON (MT M) :=
-        { raise_poison := fun A dt => lift (raise_poison dt);
-        }.
+    #[global] Instance RAISE_POISON_E_MT {M : Type -> Type} {MT : (Type -> Type) -> Type -> Type} `{MonadT (MT M) M} `{RAISE_POISON M} : RAISE_POISON (MT M) :=
+      { raise_poison := fun A dt => lift (raise_poison dt);
+      }.
 
-      Definition ErrOOMPoison := eitherT ERR_MESSAGE (eitherT OOM_MESSAGE Poisonable).
+    Definition ErrOOMPoison := eitherT ERR_MESSAGE (eitherT OOM_MESSAGE Poisonable).
 
-      Definition ErrOOMPoison_handle_poison_dv {M} `{Monad M} `{RAISE_ERROR M} `{RAISE_OOM M} (ep : ErrOOMPoison dvalue) : M dvalue
-        := match unEitherT (unEitherT ep) with
-           | Unpoisoned edv =>
-               match edv with
-               | inl (OOM_message msg) => raise_oom msg
-               | inr (inl (ERR_message msg)) => raise_error msg
-               | inr (inr val) => ret val
-               end
-           | Poison dt => ret (DVALUE_Poison dt)
-           end.
+    Definition ErrOOMPoison_handle_poison_dv {M} `{Monad M} `{RAISE_ERROR M} `{RAISE_OOM M} (ep : ErrOOMPoison dvalue) : M dvalue
+      := match unEitherT (unEitherT ep) with
+         | Unpoisoned edv =>
+             match edv with
+             | inl (OOM_message msg) => raise_oom msg
+             | inr (inl (ERR_message msg)) => raise_error msg
+             | inr (inr val) => ret val
+             end
+         | Poison dt => ret (DVALUE_Poison dt)
+         end.
 
-      (* Walk through a list *)
-      (* Returns field index + number of bytes remaining *)
-      Fixpoint extract_field_byte_helper {M} `{Monad M} `{RAISE_ERROR M} (fields : list dtyp) (field_idx : N) (byte_idx : N) : M (dtyp * (N * N))%type
-        := match fields with
-           | [] =>
-               raise_error "No fields left for byte-indexing..."
-           | (x::xs) =>
+    (* Walk through a list *)
+    (* Returns field index + number of bytes remaining *)
+    Fixpoint extract_field_byte_helper {M} `{Monad M} `{RAISE_ERROR M} (fields : list dtyp) (field_idx : N) (byte_idx : N) : M (dtyp * (N * N))%type
+      := match fields with
+         | [] =>
+             raise_error "No fields left for byte-indexing..."
+         | (x::xs) =>
              let sz := sizeof_dtyp x
              in if N.ltb byte_idx sz
                 then ret (x, (field_idx, byte_idx))
                 else extract_field_byte_helper xs (N.succ field_idx) (byte_idx - sz)
-           end.
+         end.
 
-      Definition extract_field_byte {M} `{Monad M} `{RAISE_ERROR M} (fields : list dtyp) (byte_idx : N) : M (dtyp * (N * N))%type
-        := extract_field_byte_helper fields 0 byte_idx.
+    Definition extract_field_byte {M} `{Monad M} `{RAISE_ERROR M} (fields : list dtyp) (byte_idx : N) : M (dtyp * (N * N))%type
+      := extract_field_byte_helper fields 0 byte_idx.
 
-      (* Need the type of the dvalue in order to know how big fields and array elements are.
+    (* Need the type of the dvalue in order to know how big fields and array elements are.
 
          It's not possible to use the dvalue alone, as DVALUE_Poison's
          size depends on the type.
-       *)
-      Obligation Tactic := try Tactics.program_simpl; try solve [cbn; try lia | solve_dvalue_measure].
-      Program Fixpoint dvalue_extract_byte {M} `{Monad M} `{RAISE_ERROR M} `{RAISE_POISON M} (dv : dvalue) (dt : dtyp) (idx : Z) {measure (dvalue_measure dv)} : M Z
-        := match dv with
-           | DVALUE_I1 x
-           | DVALUE_I8 x
-           | DVALUE_I32 x
-           | DVALUE_I64 x =>
-               ret (extract_byte_vint x idx)
-           | DVALUE_IPTR x =>
-               ret (extract_byte_Z (IP.to_Z x) idx)
-           | DVALUE_Addr addr =>
-               (* Note: this throws away provenance *)
-               ret (extract_byte_Z (ptr_to_int addr) idx)
-           | DVALUE_Float f =>
-               ret (extract_byte_Z (unsigned (Float32.to_bits f)) idx)
-           | DVALUE_Double d =>
-               ret (extract_byte_Z (unsigned (Float.to_bits d)) idx)
-           | DVALUE_Poison dt => raise_poison dt
-           | DVALUE_None =>
-               (* TODO: Not sure if this should be an error, poison, or what. *)
-               raise_error "dvalue_extract_byte on DVALUE_None"
+     *)
+    Obligation Tactic := try Tactics.program_simpl; try solve [cbn; try lia | solve_dvalue_measure].
+    Program Fixpoint dvalue_extract_byte {M} `{Monad M} `{RAISE_ERROR M} `{RAISE_POISON M} (dv : dvalue) (dt : dtyp) (idx : Z) {measure (dvalue_measure dv)} : M Z
+      := match dv with
+         | DVALUE_I1 x
+         | DVALUE_I8 x
+         | DVALUE_I32 x
+         | DVALUE_I64 x =>
+             ret (extract_byte_vint x idx)
+         | DVALUE_IPTR x =>
+             ret (extract_byte_Z (IP.to_Z x) idx)
+         | DVALUE_Addr addr =>
+             (* Note: this throws away provenance *)
+             ret (extract_byte_Z (ptr_to_int addr) idx)
+         | DVALUE_Float f =>
+             ret (extract_byte_Z (unsigned (Float32.to_bits f)) idx)
+         | DVALUE_Double d =>
+             ret (extract_byte_Z (unsigned (Float.to_bits d)) idx)
+         | DVALUE_Poison dt => raise_poison dt
+         | DVALUE_None =>
+             (* TODO: Not sure if this should be an error, poison, or what. *)
+             raise_error "dvalue_extract_byte on DVALUE_None"
 
-           (* TODO: Take padding into account. *)
-           | DVALUE_Struct fields =>
-               match dt with
-               | DTYPE_Struct dts =>
-                   (* Step to field which contains the byte we want *)
-                   '(fdt, (field_idx, byte_idx)) <- extract_field_byte dts (Z.to_N idx);;
-                   match List.nth_error fields (N.to_nat field_idx) with
-                   | Some f =>
-                       (* call dvalue_extract_byte recursively on the field *)
-                       dvalue_extract_byte f fdt (Z.of_N byte_idx )
-                   | None =>
-                       raise_error "dvalue_extract_byte: more fields in DVALUE_Struct than in dtyp."
-                   end
-               | _ => raise_error "dvalue_extract_byte: type mismatch on DVALUE_Struct."
-               end
+         (* TODO: Take padding into account. *)
+         | DVALUE_Struct fields =>
+             match dt with
+             | DTYPE_Struct dts =>
+                 (* Step to field which contains the byte we want *)
+                 '(fdt, (field_idx, byte_idx)) <- extract_field_byte dts (Z.to_N idx);;
+                 match List.nth_error fields (N.to_nat field_idx) with
+                 | Some f =>
+                     (* call dvalue_extract_byte recursively on the field *)
+                     dvalue_extract_byte f fdt (Z.of_N byte_idx )
+                 | None =>
+                     raise_error "dvalue_extract_byte: more fields in DVALUE_Struct than in dtyp."
+                 end
+             | _ => raise_error "dvalue_extract_byte: type mismatch on DVALUE_Struct."
+             end
 
-           | DVALUE_Packed_struct fields =>
-               match dt with
-               | DTYPE_Packed_struct dts =>
-                   (* Step to field which contains the byte we want *)
-                   '(fdt, (field_idx, byte_idx)) <- extract_field_byte dts (Z.to_N idx);;
-                   match List.nth_error fields (N.to_nat field_idx) with
-                   | Some f =>
-                       (* call dvalue_extract_byte recursively on the field *)
-                       dvalue_extract_byte f fdt (Z.of_N byte_idx )
-                   | None =>
-                       raise_error "dvalue_extract_byte: more fields in DVALUE_Packed_struct than in dtyp."
-                   end
-               | _ => raise_error "dvalue_extract_byte: type mismatch on DVALUE_Packed_struct."
-               end
+         | DVALUE_Packed_struct fields =>
+             match dt with
+             | DTYPE_Packed_struct dts =>
+                 (* Step to field which contains the byte we want *)
+                 '(fdt, (field_idx, byte_idx)) <- extract_field_byte dts (Z.to_N idx);;
+                 match List.nth_error fields (N.to_nat field_idx) with
+                 | Some f =>
+                     (* call dvalue_extract_byte recursively on the field *)
+                     dvalue_extract_byte f fdt (Z.of_N byte_idx )
+                 | None =>
+                     raise_error "dvalue_extract_byte: more fields in DVALUE_Packed_struct than in dtyp."
+                 end
+             | _ => raise_error "dvalue_extract_byte: type mismatch on DVALUE_Packed_struct."
+             end
 
-           | DVALUE_Array elts =>
-               match dt with
-               | DTYPE_Array sz dt =>
-                   let elmt_sz  := sizeof_dtyp dt in
-                   let elmt_idx := N.div (Z.to_N idx) elmt_sz in
-                   let byte_idx := (Z.to_N idx) mod elmt_sz in
-                   match List.nth_error elts (N.to_nat elmt_idx) with
-                   | Some elmt =>
-                       (* call dvalue_extract_byte recursively on the field *)
-                       dvalue_extract_byte elmt dt (Z.of_N byte_idx)
-                   | None =>
-                       raise_error "dvalue_extract_byte: more fields in dvalue than in dtyp."
-                   end
-               | _ =>
-                   raise_error "dvalue_extract_byte: type mismatch on DVALUE_Array."
-               end
+         | DVALUE_Array elts =>
+             match dt with
+             | DTYPE_Array sz dt =>
+                 let elmt_sz  := sizeof_dtyp dt in
+                 let elmt_idx := N.div (Z.to_N idx) elmt_sz in
+                 let byte_idx := (Z.to_N idx) mod elmt_sz in
+                 match List.nth_error elts (N.to_nat elmt_idx) with
+                 | Some elmt =>
+                     (* call dvalue_extract_byte recursively on the field *)
+                     dvalue_extract_byte elmt dt (Z.of_N byte_idx)
+                 | None =>
+                     raise_error "dvalue_extract_byte: more fields in dvalue than in dtyp."
+                 end
+             | _ =>
+                 raise_error "dvalue_extract_byte: type mismatch on DVALUE_Array."
+             end
 
-           | DVALUE_Vector elts =>
-               match dt with
-               | DTYPE_Vector sz dt =>
-                   let elmt_sz  := sizeof_dtyp dt in
-                   let elmt_idx := N.div (Z.to_N idx) elmt_sz in
-                   let byte_idx := (Z.to_N idx) mod elmt_sz in
-                   match List.nth_error elts (N.to_nat elmt_idx) with
-                   | Some elmt =>
-                       (* call dvalue_extract_byte recursively on the field *)
-                       dvalue_extract_byte elmt dt (Z.of_N byte_idx)
-                   | None =>
-                       raise_error "dvalue_extract_byte: more fields in dvalue than in dtyp."
-                   end
-               | _ =>
-                   raise_error "dvalue_extract_byte: type mismatch on DVALUE_Vector."
-               end
-           end.
+         | DVALUE_Vector elts =>
+             match dt with
+             | DTYPE_Vector sz dt =>
+                 let elmt_sz  := sizeof_dtyp dt in
+                 let elmt_idx := N.div (Z.to_N idx) elmt_sz in
+                 let byte_idx := (Z.to_N idx) mod elmt_sz in
+                 match List.nth_error elts (N.to_nat elmt_idx) with
+                 | Some elmt =>
+                     (* call dvalue_extract_byte recursively on the field *)
+                     dvalue_extract_byte elmt dt (Z.of_N byte_idx)
+                 | None =>
+                     raise_error "dvalue_extract_byte: more fields in dvalue than in dtyp."
+                 end
+             | _ =>
+                 raise_error "dvalue_extract_byte: type mismatch on DVALUE_Vector."
+             end
+         end.
 
-      (* Taking a byte out of a dvalue...
+    (* Taking a byte out of a dvalue...
 
       Unlike UVALUE_ExtractByte, I don't think this needs an sid
       (store id). There should be no nondeterminism in this value. *)
-      Inductive dvalue_byte : Type :=
-      | DVALUE_ExtractByte (dv : dvalue) (dt : dtyp) (idx : N) : dvalue_byte
-      .
+    Inductive dvalue_byte : Type :=
+    | DVALUE_ExtractByte (dv : dvalue) (dt : dtyp) (idx : N) : dvalue_byte
+    .
 
-      Definition dvalue_byte_value {M} `{Monad M} `{RAISE_ERROR M} `{RAISE_POISON M} (db : dvalue_byte) : M Z
-        := match db with
-           | DVALUE_ExtractByte dv dt idx =>
+    Definition dvalue_byte_value {M} `{Monad M} `{RAISE_ERROR M} `{RAISE_POISON M} (db : dvalue_byte) : M Z
+      := match db with
+         | DVALUE_ExtractByte dv dt idx =>
              dvalue_extract_byte dv dt (Z.of_N idx)
-           end.
+         end.
 
-      Obligation Tactic := try Tactics.program_simpl; try solve [cbn; try lia].
-      Program Fixpoint dvalue_bytes_to_dvalue {M} `{Monad M} `{RAISE_ERROR M} `{RAISE_POISON M} `{RAISE_OOM M} (dbs : list dvalue_byte) (dt : dtyp) {measure (dtyp_measure dt)} : M dvalue
-        := match dt with
-           | DTYPE_I sz =>
+    Obligation Tactic := try Tactics.program_simpl; try solve [cbn; try lia].
+    Program Fixpoint dvalue_bytes_to_dvalue {M} `{Monad M} `{RAISE_ERROR M} `{RAISE_POISON M} `{RAISE_OOM M} (dbs : list dvalue_byte) (dt : dtyp) {measure (dtyp_measure dt)} : M dvalue
+      := match dt with
+         | DTYPE_I sz =>
              zs <- map_monad dvalue_byte_value dbs;;
              match sz with
              | 1 =>
-               ret (DVALUE_I1 (concat_bytes_Z_vint zs))
+                 ret (DVALUE_I1 (concat_bytes_Z_vint zs))
              | 8 =>
-               ret (DVALUE_I8 (concat_bytes_Z_vint zs))
+                 ret (DVALUE_I8 (concat_bytes_Z_vint zs))
              | 32 =>
-               ret (DVALUE_I32 (concat_bytes_Z_vint zs))
+                 ret (DVALUE_I32 (concat_bytes_Z_vint zs))
              | 64 =>
-               ret (DVALUE_I64 (concat_bytes_Z_vint zs))
+                 ret (DVALUE_I64 (concat_bytes_Z_vint zs))
              | _ => raise_error "Unsupported integer size."
              end
-           | DTYPE_IPTR =>
+         | DTYPE_IPTR =>
              zs <- map_monad dvalue_byte_value dbs;;
              val <- lift_OOM (IP.from_Z (concat_bytes_Z zs));;
              ret (DVALUE_IPTR val)
-           | DTYPE_Pointer =>
+         | DTYPE_Pointer =>
              (* TODO: not sure if this should be wildcard provenance.
                 TODO: not sure if this should truncate iptr value...
               *)
              zs <- map_monad dvalue_byte_value dbs;;
              ret (DVALUE_Addr (int_to_ptr (concat_bytes_Z zs) wildcard_prov))
-           | DTYPE_Void =>
+         | DTYPE_Void =>
              raise_error "dvalue_bytes_to_dvalue on void type."
-           | DTYPE_Half =>
+         | DTYPE_Half =>
              raise_error "dvalue_bytes_to_dvalue: unsupported DTYPE_Half."
-           | DTYPE_Float =>
+         | DTYPE_Float =>
              zs <- map_monad dvalue_byte_value dbs;;
              ret (DVALUE_Float (Float32.of_bits (concat_bytes_Z_vint zs)))
-           | DTYPE_Double =>
+         | DTYPE_Double =>
              zs <- map_monad dvalue_byte_value dbs;;
              ret (DVALUE_Double (Float.of_bits (concat_bytes_Z_vint zs)))
-           | DTYPE_X86_fp80 =>
+         | DTYPE_X86_fp80 =>
              raise_error "dvalue_bytes_to_dvalue: unsupported DTYPE_X86_fp80."
-           | DTYPE_Fp128 =>
+         | DTYPE_Fp128 =>
              raise_error "dvalue_bytes_to_dvalue: unsupported DTYPE_Fp128."
-           | DTYPE_Ppc_fp128 =>
+         | DTYPE_Ppc_fp128 =>
              raise_error "dvalue_bytes_to_dvalue: unsupported DTYPE_Ppc_fp128."
-           | DTYPE_Metadata =>
+         | DTYPE_Metadata =>
              raise_error "dvalue_bytes_to_dvalue: unsupported DTYPE_Metadata."
-           | DTYPE_X86_mmx =>
+         | DTYPE_X86_mmx =>
              raise_error "dvalue_bytes_to_dvalue: unsupported DTYPE_X86_mmx."
-           | DTYPE_Array sz t =>
+         | DTYPE_Array sz t =>
              let sz := sizeof_dtyp t in
              elt_bytes <- lift_err_RAISE_ERROR (split_every sz dbs);;
              elts <- map_monad (fun es => dvalue_bytes_to_dvalue es t) elt_bytes;;
              ret (DVALUE_Array elts)
-           | DTYPE_Vector sz t =>
+         | DTYPE_Vector sz t =>
              let sz := sizeof_dtyp t in
              elt_bytes <- lift_err_RAISE_ERROR (split_every sz dbs);;
              elts <- map_monad (fun es => dvalue_bytes_to_dvalue es t) elt_bytes;;
              ret (DVALUE_Vector elts)
-           | DTYPE_Struct fields =>
+         | DTYPE_Struct fields =>
              match fields with
              | [] => ret (DVALUE_Struct []) (* TODO: Not 100% sure about this. *)
              | (dt::dts) =>
-               let sz := sizeof_dtyp dt in
-               let init_bytes := take sz dbs in
-               let rest_bytes := drop sz dbs in
-               f <- dvalue_bytes_to_dvalue init_bytes dt;;
-               rest <- dvalue_bytes_to_dvalue rest_bytes (DTYPE_Struct dts);;
-               match rest with
-               | DVALUE_Struct fs =>
-                 ret (DVALUE_Struct (f::fs))
-               | _ =>
-                 raise_error "dvalue_bytes_to_dvalue: DTYPE_Struct recursive call did not return a struct."
-               end
+                 let sz := sizeof_dtyp dt in
+                 let init_bytes := take sz dbs in
+                 let rest_bytes := drop sz dbs in
+                 f <- dvalue_bytes_to_dvalue init_bytes dt;;
+                 rest <- dvalue_bytes_to_dvalue rest_bytes (DTYPE_Struct dts);;
+                 match rest with
+                 | DVALUE_Struct fs =>
+                     ret (DVALUE_Struct (f::fs))
+                 | _ =>
+                     raise_error "dvalue_bytes_to_dvalue: DTYPE_Struct recursive call did not return a struct."
+                 end
              end
-           | DTYPE_Packed_struct fields =>
+         | DTYPE_Packed_struct fields =>
              match fields with
              | [] => ret (DVALUE_Packed_struct []) (* TODO: Not 100% sure about this. *)
              | (dt::dts) =>
-               let sz := sizeof_dtyp dt in
-               let init_bytes := take sz dbs in
-               let rest_bytes := drop sz dbs in
-               f <- dvalue_bytes_to_dvalue init_bytes dt;;
-               rest <- dvalue_bytes_to_dvalue rest_bytes (DTYPE_Struct dts);;
-               match rest with
-               | DVALUE_Packed_struct fs =>
-                 ret (DVALUE_Packed_struct (f::fs))
-               | _ =>
-                 raise_error "dvalue_bytes_to_dvalue: DTYPE_Packed_struct recursive call did not return a struct."
-               end
+                 let sz := sizeof_dtyp dt in
+                 let init_bytes := take sz dbs in
+                 let rest_bytes := drop sz dbs in
+                 f <- dvalue_bytes_to_dvalue init_bytes dt;;
+                 rest <- dvalue_bytes_to_dvalue rest_bytes (DTYPE_Struct dts);;
+                 match rest with
+                 | DVALUE_Packed_struct fs =>
+                     ret (DVALUE_Packed_struct (f::fs))
+                 | _ =>
+                     raise_error "dvalue_bytes_to_dvalue: DTYPE_Packed_struct recursive call did not return a struct."
+                 end
              end
-           | DTYPE_Opaque =>
+         | DTYPE_Opaque =>
              raise_error "dvalue_bytes_to_dvalue: unsupported DTYPE_Opaque."
-           end.
-      Next Obligation.
-        pose proof dtyp_measure_gt_0 dt.
-        cbn.
-        unfold list_sum.
-        lia.
-      Qed.
-      Next Obligation.
-        pose proof dtyp_measure_gt_0 dt.
-        cbn.
-        unfold list_sum.
-        lia.
-      Qed.
+         end.
+    Next Obligation.
+      pose proof dtyp_measure_gt_0 dt.
+      cbn.
+      unfold list_sum.
+      lia.
+    Qed.
+    Next Obligation.
+      pose proof dtyp_measure_gt_0 dt.
+      cbn.
+      unfold list_sum.
+      lia.
+    Qed.
 
-      Definition uvalue_sid_match (a b : uvalue) : bool
-        :=
-          match a, b with
-          | UVALUE_ExtractByte uv dt idx sid, UVALUE_ExtractByte uv' dt' idx' sid' =>
-            RelDec.rel_dec uv uv' && N.eqb sid sid'
-          | _, _ => false
-          end.
+    Definition uvalue_sid_match (a b : uvalue) : bool
+      :=
+      match a, b with
+      | UVALUE_ExtractByte uv dt idx sid, UVALUE_ExtractByte uv' dt' idx' sid' =>
+          RelDec.rel_dec uv uv' && N.eqb sid sid'
+      | _, _ => false
+      end.
 
-      Definition filter_uvalue_sid_matches (byte : uvalue) (uvs : list (N * uvalue)) : (list (N * uvalue) * list (N * uvalue))
-        := filter_split (fun '(n, uv) => uvalue_sid_match byte uv) uvs.
+    Definition filter_uvalue_sid_matches (byte : uvalue) (uvs : list (N * uvalue)) : (list (N * uvalue) * list (N * uvalue))
+      := filter_split (fun '(n, uv) => uvalue_sid_match byte uv) uvs.
 
-      Definition uvalue_constructor_string (u : uvalue) : string
-        := match u with
-           | UVALUE_Addr a => "UVALUE_Addr"
-           | UVALUE_I1 x => "UVALUE_I1"
-           | UVALUE_I8 x => "UVALUE_I8"
-           | UVALUE_I32 x => "UVALUE_I32"
-           | UVALUE_I64 x => "UVALUE_I64"
-           | UVALUE_IPTR x => "UVALUE_IPTR"
-           | UVALUE_Double x => "UVALUE_Double"
-           | UVALUE_Float x => "UVALUE_Float"
-           | UVALUE_Undef t => "UVALUE_Undef"
-           | UVALUE_Poison t => "UVALUE_Poison"
-           | UVALUE_None => "UVALUE_None"
-           | UVALUE_Struct fields => "UVALUE_Struct"
-           | UVALUE_Packed_struct fields => "UVALUE_Packed_struct"
-           | UVALUE_Array elts => "UVALUE_Array"
-           | UVALUE_Vector elts => "UVALUE_Vector"
-           | UVALUE_IBinop iop v1 v2 => "UVALUE_IBinop"
-           | UVALUE_ICmp cmp v1 v2 => "UVALUE_ICmp"
-           | UVALUE_FBinop fop fm v1 v2 => "UVALUE_FBinop"
-           | UVALUE_FCmp cmp v1 v2 => "UVALUE_FCmp"
-           | UVALUE_Conversion conv t_from v t_to => "UVALUE_Conversion"
-           | UVALUE_GetElementPtr t ptrval idxs => "UVALUE_GetElementPtr"
-           | UVALUE_ExtractElement vec idx => "UVALUE_ExtractElement"
-           | UVALUE_InsertElement vec elt idx => "UVALUE_InsertElement"
-           | UVALUE_ShuffleVector vec1 vec2 idxmask => "UVALUE_ShuffleVector"
-           | UVALUE_ExtractValue vec idxs => "UVALUE_ExtractValue"
-           | UVALUE_InsertValue vec elt idxs => "UVALUE_InsertValue"
-           | UVALUE_Select cnd v1 v2 => "UVALUE_Select"
-           | UVALUE_ExtractByte uv dt idx sid => "UVALUE_ExtractByte"
-           | UVALUE_ConcatBytes uvs dt => "UVALUE_ConcatBytes"
-           end.
+    Section Concretize.
+      Context (M : Type -> Type).
+      Context {HM : Monad M}.
+      Variable undef_handler : dtyp -> M dvalue.
+      Context (ERR_M : Type -> Type). (* Monad encapsulating errors, ub, oom *)
+      Context {HM_ERR : Monad ERR_M}.
+      Context {ERR : RAISE_ERROR ERR_M}.
+      Context {UB : RAISE_UB ERR_M}.
+      Context {OOM : RAISE_OOM ERR_M}.
+      Variable lift_ue : forall {A}, ERR_M A -> M A.
 
-      Section Concretize.
-        Context (M : Type -> Type).
-        Context {HM : Monad M}.
-        Variable undef_handler : dtyp -> M dvalue.
-        Context (ERR_M : Type -> Type). (* Monad encapsulating errors, ub, oom *)
-        Context {HM_ERR : Monad ERR_M}.
-        Context {ERR : RAISE_ERROR ERR_M}.
-        Context {UB : RAISE_UB ERR_M}.
-        Context {OOM : RAISE_OOM ERR_M}.
-        Variable lift_ue : forall {A}, ERR_M A -> M A.
-
-        (* TODO: satisfy the termination checker here. *)
-        (* M will be err_or_ub / MPropT err_or_ub? *)
-        Unset Guard Checking.
-        (* Define a sum type f a, g b.... a + b. Mutual recursive
+      (* TODO: satisfy the termination checker here. *)
+      (* M will be err_or_ub / MPropT err_or_ub? *)
+      Unset Guard Checking.
+      (* Define a sum type f a, g b.... a + b. Mutual recursive
            function as one big function with sum type to select between
            which "function" is being called *)
-        Fixpoint concretize_uvalueM (u : uvalue) {struct u} : M dvalue:=
-          match u with
-          | UVALUE_Addr a                          => ret (DVALUE_Addr a)
-          | UVALUE_I1 x                            => ret (DVALUE_I1 x)
-          | UVALUE_I8 x                            => ret (DVALUE_I8 x)
-          | UVALUE_I32 x                           => ret (DVALUE_I32 x)
-          | UVALUE_I64 x                           => ret (DVALUE_I64 x)
-          | UVALUE_IPTR x                          => ret (DVALUE_IPTR x)
-          | UVALUE_Double x                        => ret (DVALUE_Double x)
-          | UVALUE_Float x                         => ret (DVALUE_Float x)
-          | UVALUE_Undef t                         => undef_handler t
-          | UVALUE_Poison t                        => ret (DVALUE_Poison t)
-          | UVALUE_None                            => ret DVALUE_None
-          | UVALUE_Struct fields                   => 'dfields <- map_monad concretize_uvalueM fields ;;
-                                                     ret (DVALUE_Struct dfields)
-          | UVALUE_Packed_struct fields            => 'dfields <- map_monad concretize_uvalueM fields ;;
-                                                     ret (DVALUE_Packed_struct dfields)
-          | UVALUE_Array elts                      => 'delts <- map_monad concretize_uvalueM elts ;;
-                                                     ret (DVALUE_Array delts)
-          | UVALUE_Vector elts                     => 'delts <- map_monad concretize_uvalueM elts ;;
-                                                     ret (DVALUE_Vector delts)
-          | UVALUE_IBinop iop v1 v2                => dv1 <- concretize_uvalueM v1 ;;
-                                                     dv2 <- concretize_uvalueM v2 ;;
-                                                     lift_ue (eval_iop iop dv1 dv2)
-          | UVALUE_ICmp cmp v1 v2                  => dv1 <- concretize_uvalueM v1 ;;
-                                                     dv2 <- concretize_uvalueM v2 ;;
-                                                     lift_ue (eval_icmp cmp dv1 dv2)
-          | UVALUE_FBinop fop fm v1 v2             => dv1 <- concretize_uvalueM v1 ;;
-                                                     dv2 <- concretize_uvalueM v2 ;;
-                                                     lift_ue (eval_fop fop dv1 dv2)
-          | UVALUE_FCmp cmp v1 v2                  => dv1 <- concretize_uvalueM v1 ;;
-                                                     dv2 <- concretize_uvalueM v2 ;;
-                                                     lift_ue (eval_fcmp cmp dv1 dv2)
+      Fixpoint concretize_uvalueM (u : uvalue) {struct u} : M dvalue:=
+        match u with
+        | UVALUE_Addr a                          => ret (DVALUE_Addr a)
+        | UVALUE_I1 x                            => ret (DVALUE_I1 x)
+        | UVALUE_I8 x                            => ret (DVALUE_I8 x)
+        | UVALUE_I32 x                           => ret (DVALUE_I32 x)
+        | UVALUE_I64 x                           => ret (DVALUE_I64 x)
+        | UVALUE_IPTR x                          => ret (DVALUE_IPTR x)
+        | UVALUE_Double x                        => ret (DVALUE_Double x)
+        | UVALUE_Float x                         => ret (DVALUE_Float x)
+        | UVALUE_Undef t                         => undef_handler t
+        | UVALUE_Poison t                        => ret (DVALUE_Poison t)
+        | UVALUE_None                            => ret DVALUE_None
+        | UVALUE_Struct fields                   => 'dfields <- map_monad concretize_uvalueM fields ;;
+                                                    ret (DVALUE_Struct dfields)
+        | UVALUE_Packed_struct fields            => 'dfields <- map_monad concretize_uvalueM fields ;;
+                                                    ret (DVALUE_Packed_struct dfields)
+        | UVALUE_Array elts                      => 'delts <- map_monad concretize_uvalueM elts ;;
+                                                    ret (DVALUE_Array delts)
+        | UVALUE_Vector elts                     => 'delts <- map_monad concretize_uvalueM elts ;;
+                                                    ret (DVALUE_Vector delts)
+        | UVALUE_IBinop iop v1 v2                => dv1 <- concretize_uvalueM v1 ;;
+                                                    dv2 <- concretize_uvalueM v2 ;;
+                                                    lift_ue (eval_iop iop dv1 dv2)
+        | UVALUE_ICmp cmp v1 v2                  => dv1 <- concretize_uvalueM v1 ;;
+                                                    dv2 <- concretize_uvalueM v2 ;;
+                                                    lift_ue (eval_icmp cmp dv1 dv2)
+        | UVALUE_FBinop fop fm v1 v2             => dv1 <- concretize_uvalueM v1 ;;
+                                                    dv2 <- concretize_uvalueM v2 ;;
+                                                    lift_ue (eval_fop fop dv1 dv2)
+        | UVALUE_FCmp cmp v1 v2                  => dv1 <- concretize_uvalueM v1 ;;
+                                                    dv2 <- concretize_uvalueM v2 ;;
+                                                    lift_ue (eval_fcmp cmp dv1 dv2)
 
-          | UVALUE_Conversion conv t_from v t_to    =>
+        | UVALUE_Conversion conv t_from v t_to    =>
             dv <- concretize_uvalueM v ;;
             match get_conv_case conv t_from dv t_to with
             | Conv_PtoI x =>
-              match x, t_to with
-              | DVALUE_Addr addr, DTYPE_I sz =>
-                lift_ue (coerce_integer_to_int (Some sz) (ptr_to_int addr))
-              | DVALUE_Addr addr, DTYPE_IPTR =>
-                lift_ue (coerce_integer_to_int None (ptr_to_int addr))
-              | _, _ =>
-                lift_ue (raise_error "Invalid PTOI conversion")
-              end
+                match x, t_to with
+                | DVALUE_Addr addr, DTYPE_I sz =>
+                    lift_ue (coerce_integer_to_int (Some sz) (ptr_to_int addr))
+                | DVALUE_Addr addr, DTYPE_IPTR =>
+                    lift_ue (coerce_integer_to_int None (ptr_to_int addr))
+                | _, _ =>
+                    lift_ue (raise_error "Invalid PTOI conversion")
+                end
             | Conv_ItoP x => ret (DVALUE_Addr (int_to_ptr (dvalue_int_unsigned x) wildcard_prov))
             | Conv_Pure x => ret x
             | Conv_Illegal s => lift_ue (raise_error s)
             end
 
-          | UVALUE_GetElementPtr t ua uvs =>
+        | UVALUE_GetElementPtr t ua uvs =>
             da <- concretize_uvalueM ua;;
             dvs <- map_monad concretize_uvalueM uvs;;
             match handle_gep t da dvs with
@@ -873,65 +835,65 @@ Module Make(Addr:MemoryAddress.ADDRESS)(IP:MemoryAddress.INTPTR)(SIZEOF: Sizeof)
             | inl err => lift_ue (raise_error err)
             end
 
-          | UVALUE_ExtractValue uv idxs =>
+        | UVALUE_ExtractValue uv idxs =>
             str <- concretize_uvalueM uv;;
             let fix loop str idxs : ERR_M dvalue :=
-                match idxs with
-                | [] => ret str
-                | i :: tl =>
+              match idxs with
+              | [] => ret str
+              | i :: tl =>
                   v <- index_into_str_dv str i ;;
                   loop v tl
-                end in
+              end in
             lift_ue (loop str idxs)
 
-          | UVALUE_Select cond v1 v2 =>
+        | UVALUE_Select cond v1 v2 =>
             dcond <- concretize_uvalueM cond;;
             uv <- lift_ue (eval_select dcond v1 v2);;
             concretize_uvalueM uv
 
-          | UVALUE_ConcatBytes bytes dt =>
+        | UVALUE_ConcatBytes bytes dt =>
             match N.eqb (N.of_nat (length bytes)) (sizeof_dtyp dt), all_extract_bytes_from_uvalue bytes with
             | true, Some uv => concretize_uvalueM uv
             | _, _ => extractbytes_to_dvalue bytes dt
             end
 
-          | UVALUE_ExtractByte byte dt idx sid =>
+        | UVALUE_ExtractByte byte dt idx sid =>
             (* TODO: maybe this is just an error? ExtractByte should be guarded by ConcatBytes? *)
             lift_ue (raise_error "Attempting to concretize UVALUE_ExtractByte, should not happen.")
 
-          | _ => lift_ue (raise_error ("concretize_uvalueM: Attempting to convert a partially non-reduced uvalue to dvalue. Should not happen: " ++ uvalue_constructor_string u))
+        | _ => lift_ue (raise_error ("concretize_uvalueM: Attempting to convert a partially non-reduced uvalue to dvalue. Should not happen: " ++ uvalue_constructor_string u))
 
-          end
+        end
 
-        with
+      with
 
-        (* Take a UVALUE_ExtractByte, and replace the uvalue with a given dvalue...
+      (* Take a UVALUE_ExtractByte, and replace the uvalue with a given dvalue...
 
          Note: this also concretizes the index.
-         *)
-        uvalue_byte_replace_with_dvalue_byte (uv : uvalue) (dv : dvalue) {struct uv} : M dvalue_byte
-          := match uv with
-             | UVALUE_ExtractByte uv dt idx sid =>
-               cidx <- concretize_uvalueM idx;;
-               ret (DVALUE_ExtractByte dv dt (Z.to_N (dvalue_int_unsigned cidx)))
-             | _ => lift_ue (raise_error "uvalue_byte_replace_with_dvalue_byte called with non-UVALUE_ExtractByte value.")
-             end
+       *)
+      uvalue_byte_replace_with_dvalue_byte (uv : uvalue) (dv : dvalue) {struct uv} : M dvalue_byte
+      := match uv with
+         | UVALUE_ExtractByte uv dt idx sid =>
+             cidx <- concretize_uvalueM idx;;
+             ret (DVALUE_ExtractByte dv dt (Z.to_N (dvalue_int_unsigned cidx)))
+         | _ => lift_ue (raise_error "uvalue_byte_replace_with_dvalue_byte called with non-UVALUE_ExtractByte value.")
+         end
 
-        with
-        (* Concretize the uvalues in a list of UVALUE_ExtractBytes...
+      with
+      (* Concretize the uvalues in a list of UVALUE_ExtractBytes...
 
-         *)
-        (* Pick out uvalue bytes that are the same + have same sid
+       *)
+      (* Pick out uvalue bytes that are the same + have same sid
 
          Concretize these identical uvalues...
-         *)
+       *)
 
-        concretize_uvalue_bytes_helper (uvs : list (N * uvalue)) (acc : NMap dvalue_byte) {struct uvs} : M (NMap dvalue_byte)
-          := match uvs with
-             | [] => ret acc
-             | ((n, uv)::uvs) =>
-               match uv with
-               | UVALUE_ExtractByte byte_uv dt idx sid =>
+      concretize_uvalue_bytes_helper (uvs : list (N * uvalue)) (acc : NMap dvalue_byte) {struct uvs} : M (NMap dvalue_byte)
+      := match uvs with
+         | [] => ret acc
+         | ((n, uv)::uvs) =>
+             match uv with
+             | UVALUE_ExtractByte byte_uv dt idx sid =>
                  let '(ins, outs) := filter_uvalue_sid_matches uv uvs in
                  (* Concretize first uvalue *)
                  dv <- concretize_uvalueM byte_uv;;
@@ -940,289 +902,133 @@ Module Make(Addr:MemoryAddress.ADDRESS)(IP:MemoryAddress.INTPTR)(SIZEOF: Sizeof)
                  let acc := @NM.add _ n dv_byte acc in
                  (* Concretize entangled bytes *)
                  acc <- monad_fold_right (fun acc '(n, uv) =>
-                                           dvb <- uvalue_byte_replace_with_dvalue_byte uv dv;;
-                                           ret (@NM.add _ n dvb acc)) ins acc;;
+                                            dvb <- uvalue_byte_replace_with_dvalue_byte uv dv;;
+                                            ret (@NM.add _ n dvb acc)) ins acc;;
                  (* Concretize the rest of the bytes *)
                  concretize_uvalue_bytes_helper outs acc
-               | _ => lift_ue (raise_error "concretize_uvalue_bytes_helper: non-byte in uvs.")
-               end
+             | _ => lift_ue (raise_error "concretize_uvalue_bytes_helper: non-byte in uvs.")
              end
+         end
 
-        with
-        concretize_uvalue_bytes (uvs : list uvalue) {struct uvs} : M (list dvalue_byte)
-          :=
-            let len := length uvs in
-            byte_map <- concretize_uvalue_bytes_helper (zip (Nseq 0 len) uvs) (@NM.empty _);;
-            match NM_find_many (Nseq 0 len) byte_map with
-            | Some dvbs => ret dvbs
-            | None => lift_ue (raise_error "concretize_uvalue_bytes: missing indices.")
-            end
+      with
+      concretize_uvalue_bytes (uvs : list uvalue) {struct uvs} : M (list dvalue_byte)
+      :=
+        let len := length uvs in
+        byte_map <- concretize_uvalue_bytes_helper (zip (Nseq 0 len) uvs) (@NM.empty _);;
+        match NM_find_many (Nseq 0 len) byte_map with
+        | Some dvbs => ret dvbs
+        | None => lift_ue (raise_error "concretize_uvalue_bytes: missing indices.")
+        end
 
-        with
-        extractbytes_to_dvalue (uvs : list uvalue) (dt : dtyp) {struct uvs} : M dvalue
-          := dvbs <- concretize_uvalue_bytes uvs;;
-             lift_ue (ErrOOMPoison_handle_poison_dv (dvalue_bytes_to_dvalue dvbs dt)).
+      with
+      extractbytes_to_dvalue (uvs : list uvalue) (dt : dtyp) {struct uvs} : M dvalue
+      := dvbs <- concretize_uvalue_bytes uvs;;
+         lift_ue (ErrOOMPoison_handle_poison_dv (dvalue_bytes_to_dvalue dvbs dt)).
 
-        Lemma concretize_uvalueM_equation :
-          forall u,
-            concretize_uvalueM u =
-          match u with
-          | UVALUE_Addr a                          => ret (DVALUE_Addr a)
-          | UVALUE_I1 x                            => ret (DVALUE_I1 x)
-          | UVALUE_I8 x                            => ret (DVALUE_I8 x)
-          | UVALUE_I32 x                           => ret (DVALUE_I32 x)
-          | UVALUE_I64 x                           => ret (DVALUE_I64 x)
-          | UVALUE_IPTR x                          => ret (DVALUE_IPTR x)
-          | UVALUE_Double x                        => ret (DVALUE_Double x)
-          | UVALUE_Float x                         => ret (DVALUE_Float x)
-          | UVALUE_Undef t                         => undef_handler t
-          | UVALUE_Poison t                        => ret (DVALUE_Poison t)
-          | UVALUE_None                            => ret DVALUE_None
-          | UVALUE_Struct fields                   => 'dfields <- map_monad concretize_uvalueM fields ;;
-                                                     ret (DVALUE_Struct dfields)
-          | UVALUE_Packed_struct fields            => 'dfields <- map_monad concretize_uvalueM fields ;;
-                                                     ret (DVALUE_Packed_struct dfields)
-          | UVALUE_Array elts                      => 'delts <- map_monad concretize_uvalueM elts ;;
-                                                     ret (DVALUE_Array delts)
-          | UVALUE_Vector elts                     => 'delts <- map_monad concretize_uvalueM elts ;;
-                                                     ret (DVALUE_Vector delts)
-          | UVALUE_IBinop iop v1 v2                => dv1 <- concretize_uvalueM v1 ;;
-                                                     dv2 <- concretize_uvalueM v2 ;;
-                                                     lift_ue (eval_iop iop dv1 dv2)
-          | UVALUE_ICmp cmp v1 v2                  => dv1 <- concretize_uvalueM v1 ;;
-                                                     dv2 <- concretize_uvalueM v2 ;;
-                                                     lift_ue (eval_icmp cmp dv1 dv2)
-          | UVALUE_FBinop fop fm v1 v2             => dv1 <- concretize_uvalueM v1 ;;
-                                                     dv2 <- concretize_uvalueM v2 ;;
-                                                     lift_ue (eval_fop fop dv1 dv2)
-          | UVALUE_FCmp cmp v1 v2                  => dv1 <- concretize_uvalueM v1 ;;
-                                                     dv2 <- concretize_uvalueM v2 ;;
-                                                     lift_ue (eval_fcmp cmp dv1 dv2)
+      Lemma concretize_uvalueM_equation :
+        forall u,
+          concretize_uvalueM u =
+            match u with
+            | UVALUE_Addr a                          => ret (DVALUE_Addr a)
+            | UVALUE_I1 x                            => ret (DVALUE_I1 x)
+            | UVALUE_I8 x                            => ret (DVALUE_I8 x)
+            | UVALUE_I32 x                           => ret (DVALUE_I32 x)
+            | UVALUE_I64 x                           => ret (DVALUE_I64 x)
+            | UVALUE_IPTR x                          => ret (DVALUE_IPTR x)
+            | UVALUE_Double x                        => ret (DVALUE_Double x)
+            | UVALUE_Float x                         => ret (DVALUE_Float x)
+            | UVALUE_Undef t                         => undef_handler t
+            | UVALUE_Poison t                        => ret (DVALUE_Poison t)
+            | UVALUE_None                            => ret DVALUE_None
+            | UVALUE_Struct fields                   => 'dfields <- map_monad concretize_uvalueM fields ;;
+                                                        ret (DVALUE_Struct dfields)
+            | UVALUE_Packed_struct fields            => 'dfields <- map_monad concretize_uvalueM fields ;;
+                                                        ret (DVALUE_Packed_struct dfields)
+            | UVALUE_Array elts                      => 'delts <- map_monad concretize_uvalueM elts ;;
+                                                        ret (DVALUE_Array delts)
+            | UVALUE_Vector elts                     => 'delts <- map_monad concretize_uvalueM elts ;;
+                                                        ret (DVALUE_Vector delts)
+            | UVALUE_IBinop iop v1 v2                => dv1 <- concretize_uvalueM v1 ;;
+                                                        dv2 <- concretize_uvalueM v2 ;;
+                                                        lift_ue (eval_iop iop dv1 dv2)
+            | UVALUE_ICmp cmp v1 v2                  => dv1 <- concretize_uvalueM v1 ;;
+                                                        dv2 <- concretize_uvalueM v2 ;;
+                                                        lift_ue (eval_icmp cmp dv1 dv2)
+            | UVALUE_FBinop fop fm v1 v2             => dv1 <- concretize_uvalueM v1 ;;
+                                                        dv2 <- concretize_uvalueM v2 ;;
+                                                        lift_ue (eval_fop fop dv1 dv2)
+            | UVALUE_FCmp cmp v1 v2                  => dv1 <- concretize_uvalueM v1 ;;
+                                                        dv2 <- concretize_uvalueM v2 ;;
+                                                        lift_ue (eval_fcmp cmp dv1 dv2)
 
-          | UVALUE_Conversion conv t_from v t_to    =>
-            dv <- concretize_uvalueM v ;;
-            match get_conv_case conv t_from dv t_to with
-            | Conv_PtoI x =>
-              match x, t_to with
-              | DVALUE_Addr addr, DTYPE_I sz =>
-                lift_ue (coerce_integer_to_int (Some sz) (ptr_to_int addr))
-              | DVALUE_Addr addr, DTYPE_IPTR =>
-                lift_ue (coerce_integer_to_int None (ptr_to_int addr))
-              | _, _ =>
-                lift_ue (raise_error "Invalid PTOI conversion")
-              end
-            | Conv_ItoP x => ret (DVALUE_Addr (int_to_ptr (dvalue_int_unsigned x) wildcard_prov))
-            | Conv_Pure x => ret x
-            | Conv_Illegal s => lift_ue (raise_error s)
-            end
+            | UVALUE_Conversion conv t_from v t_to    =>
+                dv <- concretize_uvalueM v ;;
+                match get_conv_case conv t_from dv t_to with
+                | Conv_PtoI x =>
+                    match x, t_to with
+                    | DVALUE_Addr addr, DTYPE_I sz =>
+                        lift_ue (coerce_integer_to_int (Some sz) (ptr_to_int addr))
+                    | DVALUE_Addr addr, DTYPE_IPTR =>
+                        lift_ue (coerce_integer_to_int None (ptr_to_int addr))
+                    | _, _ =>
+                        lift_ue (raise_error "Invalid PTOI conversion")
+                    end
+                | Conv_ItoP x => ret (DVALUE_Addr (int_to_ptr (dvalue_int_unsigned x) wildcard_prov))
+                | Conv_Pure x => ret x
+                | Conv_Illegal s => lift_ue (raise_error s)
+                end
 
-          | UVALUE_GetElementPtr t ua uvs =>
-            da <- concretize_uvalueM ua;;
-            dvs <- map_monad concretize_uvalueM uvs;;
-            match handle_gep t da dvs with
-            | inr dv  => ret dv
-            | inl err => lift_ue (raise_error err)
-            end
+            | UVALUE_GetElementPtr t ua uvs =>
+                da <- concretize_uvalueM ua;;
+                dvs <- map_monad concretize_uvalueM uvs;;
+                match handle_gep t da dvs with
+                | inr dv  => ret dv
+                | inl err => lift_ue (raise_error err)
+                end
 
-          | UVALUE_ExtractValue uv idxs =>
-            str <- concretize_uvalueM uv;;
-            let fix loop str idxs : ERR_M dvalue :=
-                match idxs with
-                | [] => ret str
-                | i :: tl =>
-                  v <- index_into_str_dv str i ;;
-                  loop v tl
-                end in
-            lift_ue (loop str idxs)
+            | UVALUE_ExtractValue uv idxs =>
+                str <- concretize_uvalueM uv;;
+                let fix loop str idxs : ERR_M dvalue :=
+                  match idxs with
+                  | [] => ret str
+                  | i :: tl =>
+                      v <- index_into_str_dv str i ;;
+                      loop v tl
+                  end in
+                lift_ue (loop str idxs)
 
-          | UVALUE_Select cond v1 v2 =>
-            dcond <- concretize_uvalueM cond;;
-            uv <- lift_ue (eval_select dcond v1 v2);;
-            concretize_uvalueM uv
+            | UVALUE_Select cond v1 v2 =>
+                dcond <- concretize_uvalueM cond;;
+                uv <- lift_ue (eval_select dcond v1 v2);;
+                concretize_uvalueM uv
 
-          | UVALUE_ConcatBytes bytes dt =>
-            match N.eqb (N.of_nat (length bytes)) (sizeof_dtyp dt), all_extract_bytes_from_uvalue bytes with
-            | true, Some uv => concretize_uvalueM uv
-            | _, _ => extractbytes_to_dvalue bytes dt
-            end
+            | UVALUE_ConcatBytes bytes dt =>
+                match N.eqb (N.of_nat (length bytes)) (sizeof_dtyp dt), all_extract_bytes_from_uvalue bytes with
+                | true, Some uv => concretize_uvalueM uv
+                | _, _ => extractbytes_to_dvalue bytes dt
+                end
 
-          | UVALUE_ExtractByte byte dt idx sid =>
-            (* TODO: maybe this is just an error? ExtractByte should be guarded by ConcatBytes? *)
-            lift_ue (raise_error "Attempting to concretize UVALUE_ExtractByte, should not happen.")
+            | UVALUE_ExtractByte byte dt idx sid =>
+                (* TODO: maybe this is just an error? ExtractByte should be guarded by ConcatBytes? *)
+                lift_ue (raise_error "Attempting to concretize UVALUE_ExtractByte, should not happen.")
 
-          | _ => lift_ue (raise_error ("concretize_uvalueM: Attempting to convert a partially non-reduced uvalue to dvalue. Should not happen: " ++ uvalue_constructor_string u))
+            | _ => lift_ue (raise_error ("concretize_uvalueM: Attempting to convert a partially non-reduced uvalue to dvalue. Should not happen: " ++ uvalue_constructor_string u))
 
-          end.
-        Proof.
-          intros u.
-          unfold concretize_uvalueM.
-          destruct u; try reflexivity.
-        Qed.
-
-        Set Guard Checking.
-      End Concretize.
-
-      Arguments concretize_uvalueM {_ _}.
-
-      Definition concretize_uvalue {M} `{Monad M} `{RAISE_ERROR M} `{RAISE_UB M} `{RAISE_OOM M}
-                 (uv : uvalue) : M dvalue
-        := concretize_uvalueM (fun dt => lift_err_RAISE_ERROR (default_dvalue_of_dtyp dt)) _ _ _ _ _ (fun _ x => x) uv.
-
-      Definition concretize_u (uv : uvalue) : RefineProp dvalue.
-        refine (concretize_uvalueM
-                  (fun dt => _)
-                  err_ub_oom
-                  _
-                  _
-                  _
-                  _
-                  (fun _ x => _) uv).
-
-        (* Undef handler *)
-        { unfold RefineProp.
-          refine (fun edv => match unERR_UB_OOM edv with
-                          | mkEitherT (mkEitherT (mkEitherT (mkIdent (inr (inr (inr dv)))))) =>
-                              (* As long as the dvalue has the same type, it's a refinement *)
-                              dvalue_has_dtyp dv dt
-                          | _ => False
-                          end).
-        }
-
-        (* lift_ue *)
-        { unfold RefineProp.
-          intros ue.
-
-          (* Is x or ue the thing that should be the refinement? *)
-          (* I think ue is the refinement *)
-          destruct x as [[[[[[[oom_x] | [[ub_x] | [[err_x] | x]]]]]]]].
-          - (* OOM *)
-            (* OOM only refines OOM *)
-            destruct ue as [[[[[[[oom_ue] | [[ub_ue] | [[err_ue] | ue]]]]]]]].
-            + exact True.
-            + exact False.
-            + exact False.
-            + exact False.
-          - (* UB *)
-            exact True.
-          - (* ERR *)
-            exact True.
-          - destruct ue as [[[[[[[oom_ue] | [[ub_ue] | [[err_ue] | ue]]]]]]]].
-            + exact True. (* OOM refines everything *)
-            + exact False.
-            + exact False.
-            + exact (x = ue).
-        }
-      Defined.
-
-      Definition concretize_u_succeeds (uv : uvalue) : RefineProp dvalue.
-        refine (concretize_uvalueM (fun dt => _)
-                                   err_ub_oom
-                                   _
-                                   _
-                                   _
-                                   _
-                                   (fun _ x => _) uv).
-
-        (* Undef handler *)
-        { unfold RefineProp.
-          refine (fun edv => match unERR_UB_OOM edv with
-                    | mkEitherT (mkEitherT (mkEitherT (mkIdent (inr (inr (inr dv)))))) =>
-                      (* As long as the dvalue has the same type, it's a refinement *)
-                      dvalue_has_dtyp dv dt
-                    | _ => False
-                    end).
-        }
-
-        (* lift_ue *)
-        { unfold RefineProp.
-          intros ue.
-
-          exact (~MFails x /\ ~MFails ue).
-        }
-      Defined.
-
-      Definition concretize (uv: uvalue) (dv : dvalue) := concretize_u uv (ret dv).
-
-      Definition concretize_fails (uv : uvalue) : Prop
-        := concretize_u uv (raise_ub "").
-
-      Definition concretize_succeeds (uv : uvalue) : Prop
-        := ~ concretize_fails uv.
-
-      Lemma concretize_equation : forall (uv: uvalue) (dv : dvalue),
-          concretize uv dv = concretize_u uv (ret dv).
+            end.
       Proof.
-        reflexivity.
+        intros u.
+        unfold concretize_uvalueM.
+        destruct u; try reflexivity.
       Qed.
 
-      Lemma Concretize_Undef : forall dt dv,
-          dvalue_has_dtyp dv dt ->
-          concretize (UVALUE_Undef dt) dv.
-      Proof.
-        intros dt dv H.
-        rewrite concretize_equation.
-        unfold concretize_u.
-        red; cbn; auto.
-      Qed.
-
-      Lemma Concretize_IBinop : forall iop uv1 e1 uv2 e2,
-          concretize_u uv1 e1 ->
-          concretize_u uv2 e2 ->
-          concretize_u (UVALUE_IBinop iop uv1 uv2)
-                       (dv1 <- e1 ;;
-                        dv2 <- e2 ;;
-                        (eval_iop iop dv1 dv2)).
-      Proof.
-        intros iop uv1 e1 uv2 e2 C1 C2.
-        unfold concretize_u in *.
-
-        rewrite concretize_uvalueM_equation.
-        red.
-
-        unfold bind.
-        cbn.
-        unfold bind_RefineProp.
-
-        eexists.
-        exists (fun x => match unIdent (unEitherT (unEitherT (unEitherT (unERR_UB_OOM e2)))) with
-                 | inl (OOM_message oom) => raise_oom oom
-                 | inr (inl (UB_message ub)) => raise_ub ub
-                 | inr (inr (inl (ERR_message err))) => raise_error err
-                 | inr (inr (inr x0)) => eval_iop iop x x0
-                 end).
-        split; eauto.
-        split.
-
-        { (* Monad.eq1 mb (x <- ma;; k' x) *)
-          unfold bind.
-          cbn.
-          destruct e1 as [[[[[[[oom_e1] | [[ub_e1] | [[err_e1] | e1]]]]]]]]; cbn; try reflexivity.
-          destruct e2 as [[[[[[[oom_e2] | [[ub_e2] | [[err_e2] | e2]]]]]]]]; cbn; try reflexivity.
-
-          destruct (eval_iop iop e1 e2) as [[[[[[[oom_eval_iopiope1e2] | [[ub_eval_iopiope1e2] | [[err_eval_iopiope1e2] | eval_iopiope1e2]]]]]]]]; reflexivity.
-        }
-
-        right.
-        intros dv1 Re1.
-
-        eexists.
-        exists (fun x0 => eval_iop iop dv1 x0).
-        split; eauto.
-        split.
-
-        { (* Monad.eq1 mb (x <- ma;; k' x) *)
-          unfold bind.
-          cbn.
-          destruct e2 as [[[[[[[oom_e2] | [[ub_e2] | [[err_e2] | e2]]]]]]]]; cbn; try reflexivity.
-
-          unfold Monad.eq1.
-          destruct (eval_iop iop dv1 e2) as [[[[[[[oom_eval_iopiopdv1e2] | [[ub_eval_iopiopdv1e2] | [[err_eval_iopiopdv1e2] | eval_iopiopdv1e2]]]]]]]]; reflexivity.
-        }
-
-        right.
-        intros dv2 Re2.
-        destruct (eval_iop iop dv1 dv2) as [[[[[[[oom_eval_iopiopdv1dv2] | [[ub_eval_iopiopdv1dv2] | [[err_eval_iopiopdv1dv2] | eval_iopiopdv1dv2]]]]]]]]; reflexivity.
-      Qed.
-
+      Set Guard Checking.
     End Concretize.
+
+    Arguments concretize_uvalueM {_ _}.
+
+  End Concretize.
+End MakeBase.
+
+Module Make (LP : LLVMParams) (Events : LLVM_INTERACTIONS LP.ADDR LP.IP LP.SIZEOF) (MP : MemoryParams LP Events) (SER : SerializationBase LP Events MP) : Serialization LP Events MP SER.
+  Include Serialization LP Events MP SER.
 End Make.
